Test/Builtin/attributes.mlir
@@ -8,10 +8,16 @@
   %6 = "test.test"() <{unregistered = #unregistered.dialect<foo 3 + 2>}> : () -> i32
   %7 = "test.test"() <{u = unit}> : () -> i32
   %8 = "test.test"() <{u}> : () -> i32
+  %9 = "test.test"() <{dict = {a = 0 : i32, b = "hello"}}> : () -> i32
+  %10 = "test.test"() <{empty_dict = {}}> : () -> i32
+  %11 = "test.test"() <{dict_unit = {x, y}}> : () -> i32
 }) : () -> ()
 
 // CHECK-NEXT: "builtin.module"() ({
 // CHECK-NEXT:   ^{{.*}}():
+// CHECK-NEXT:     %{{.*}} = "test.test"() : () -> i32
+// CHECK-NEXT:     %{{.*}} = "test.test"() : () -> i32
+// CHECK-NEXT:     %{{.*}} = "test.test"() : () -> i32
 // CHECK-NEXT:     %{{.*}} = "test.test"() : () -> i32
 // CHECK-NEXT:     %{{.*}} = "test.test"() : () -> i32
 // CHECK-NEXT:     %{{.*}} = "test.test"() : () -> i32
